Let us first assume that there is no regeneration ($\rho = \frac{T_A}{T_R} = 0$), which is a sensible thing to do since most of the time $T_A \ll T_R$. This reduces the transition matrix into a triangular one making an exact analytic solution using forward substitution possible. The effects of overkill still remain which makes such an approximation interesting.

We begin by restating the regenerationless transition probabilities
\begin{align}
	\pi_{i,j} = \begin{cases}
		\Pr{X = i-j}, &\mbox{if } j > 0 \\
		\Pr{X \geq i-j}, &\mbox{if } j = 0
	\end{cases}
\end{align}
where
\begin{align}
	\Pr{X=n} = \begin{cases}
		1 - \frac{am}{m+1}, &\mbox{if } n = 0 \\
		\frac{a}{m+1},      &\mbox{if } 1 \leq n \leq m\\
		0,      			&\mbox{if } n > m\ \mbox{or } n < 0.
	\end{cases}
\end{align}
Obviously, $\E{R_i} = 0$ because there is no regeneration, so it suffices to find the expected length of a fight $\E{L_i}$. Note that since there is now no way for the remaining hitpoints of the enemy to transition upwards, a fight against an enemy with $i$ hitpoints remaining is equivalent to one against an enemy for which $i$ is the maximum hitpoints. Therefore, we can without loss of generality assume that the initial state is $h$.
The now triangular transition matrix allows solving for $\E{L_i}$ recursively. To do this we write the matrix equation~(\ref{eq:fightLengthMatrix}) explicitly.
\begin{align*}
	\mathbf{1} &= (\mathbf{I} - \mathbf{Q})\mathbf{L}\\
	\implies 1 &= \sum_{j=1}^h(\delta_{h,j} - \pi_{h,j})\E{L_j}\\
		&= (1 - \pi_{h,h})\E{L_h} - \sum_{j=1}^{h-1} \pi_{h,j}\E{L_j}\\
		&= \big(1 - \Pr{X=0}\big)\E{L_h} - \sum_{j=1}^{h-1} \Pr{X=h-j}\E{L_j}\\
		&= \frac{am}{m+1}\E{L_h} - \sum_{j=h-m}^{h-1} \frac{a}{m+1}\E{L_j}\\
	\implies \frac{am}{m+1}\E{L_h}
		&= 1 + \frac{a}{m+1}\sum_{j=h-m}^{h-1} \E{L_j}
\end{align*}
To simplify the summation limits, we have defined $\E{L_i} = 0$ for $i \leq 0$. Finally, after reversing the order of summation and multiplying by $\frac{m+1}{am}$ the recurrence relation becomes
\begin{align}
	\E{L_h} = \E{L_1} + \frac{1}{m}\sum_{j=1}^m \E{L_{h-j}}\label{eq:noregenRecursion}
\end{align}
where $\E{L_1} = \frac{m+1}{am}$ as discussed in Chapter~\ref{chap:fightLength}.
