\subsection{Recurrence relations}
Inserting the transition probabilities into eq\ref{eq:fightLengthRecursion} gives
\begin{align}
    \langle L_h \rangle
        &= 1 + \sum_{i=1}^h \Pr{X=\,h-i}\langle L_i\rangle\nonumber\\
        &= 1 + \Pr{X=\,0}\langle L_h \rangle + \sum_{i=1}^{h-1} \Pr{X=\,h-i}\langle L_i \rangle\nonumber\\
    \implies \left(1 - \Pr{X=\,0}\right)\langle L_h \rangle &= 1 + \sum_{i=1}^{h-1} \Pr{X=\,h-i}\langle L_i \rangle\label{eq:noregen1}
\end{align}
Now there are three cases to be considered.\\
\textbf{Case:} $h = 1$
\begin{align}
	\langle L_1 \rangle = \frac{1}{1-\Pr{X=\,0}} = \frac{m+1}{am}
\end{align}
\textbf{Case:} $1 < h \leq m+1$
\begin{align}
	\langle L_h \rangle
		&= \frac{m + 1}{am} + \frac{m+1}{am} \sum_{i=1}^{h-1}\frac{a}{m+1}\langle L_{i} \rangle\nonumber\\
		&= \langle L_{1} \rangle + \frac{1}{m} \sum_{i=1}^{h-1}\langle L_{i} \rangle\nonumber\\
		&= \underbrace{\langle L_{1} \rangle + \frac{1}{m} \sum_{i=1}^{h-2}\langle L_{i} \rangle}_{\langle L_{h-1}\rangle} +\,\frac{1}{m}\langle L_{h-1} \rangle\nonumber\\
		&= \frac{m+1}{m}\langle L_{h-1}\rangle\label{eq:geometricRecurrence}
\end{align}
\textbf{Case:} $h > m+1$
\begin{align}
    \langle L_h \rangle
        &= \langle L_{1} \rangle + \frac{1}{m}\sum_{i=h-1-m}^{\mathclap{h-1}} \langle L_i \rangle\nonumber\\
		&= \underbrace{\langle L_{1} \rangle + \frac{1}{m}\sum_{i=h-2-m}^{h-2} \langle L_i \rangle}_{\langle L_{h-1}\rangle} +\,\frac{1}{m}\langle L_{h-1} \rangle - \frac{1}{m}\langle L_{h-m-1} \rangle\nonumber\\
    	&= \frac{m+1}{m}\langle L_{h-1} \rangle - \frac{1}{m}\langle L_{h-m-1} \rangle\nonumber\\
		&= \frac{m+1}{m}\left(\langle L_{h-1} \rangle - \frac{1}{m+1}\langle L_{h-m-1} \rangle\right) \label{eq:complexRecurrence}
\end{align}

